src/tls/Hashing.fst
@@ -1,86 +1,47 @@
-﻿(** hash algorithms and providers *)
 module Hashing
 
-// this file to be split into several once it moves to HACL*
-
-//________________ Hash.Spec __________________
+open FStar.Heap
+open FStar.HyperHeap
+open FStar.HyperStack
 
 open Platform.Bytes
+open Hashing.Spec
 
-type alg = // CoreCrypto.hash_alg
-  | MD5
-  | SHA1
-  | SHA224
-  | SHA256
-  | SHA384
-  | SHA512
+(* IMPLEMENTATION PLACEHOLDER, 
+    simply buffering the bytes underneath *)
 
-// see e.g. https://en.wikipedia.org/wiki/SHA-1 for a global comparison
+//17-01-26 ??? abstract 
+type accv (a:alg) =  | Inputs: bytes -> accv a
+val content: #a:alg -> accv a -> Tot bytes 
+let content #a v = 
+  match v with Inputs b -> b
 
-// length of the input blocks, in bytes (used for specifying the outer hash loop)
-let blockLen = function 
-  | MD5 | SHA1 | SHA224 | SHA256 -> 64 
-  | SHA384 | SHA512 -> 128
+val start: a:alg -> Tot (v:accv a {content v == empty_bytes})
+val extend: #a:alg -> v:accv a -> b:bytes -> Tot (v':accv a {content v' == content v @| b})
+val finalize: #a:alg -> v:accv a -> ST (t:tag a {t == hash a (content v)})
+  (requires (fun h0 -> True))
+  (ensures (fun h0 t h1 -> modifies Set.empty h0 h1))
 
-// length of the resulting tag, in bytes (replicating CoreCrypto.hashSize)
-let tagLen = function 
-  | MD5      -> 16
-  | SHA1     -> 20
-  | SHA224 -> 28 // truncated SHA256
-  | SHA256 -> 32
-  | SHA384 -> 48 // truncated SHA512
-  | SHA512 -> 64 
+let start a = Inputs empty_bytes
+let extend #a (Inputs b0) b1 = Inputs (b0 @| b1)
+let finalize #a (Inputs b) = Hashing.OpenSSL.compute a b
 
-// internal hash state for incremental computation
-assume type acc (a:alg)
-assume val acc0: a:alg -> Tot (acc a)
-(*
-let acc0 = function 
-  | MD5 ->  [0x67452301; 0xefcdab89; 0x98badcfe; 0x10325476] // A, B, C, D
-  | SHA1 -> [0x67452301; 0xefcdab89; 0x98badcfe; 0x10325476; 0xc3d2e1f0] // h0--h4 
-  | SHA224 -> [0xc1059ed8; 0x367cd507; 0x3070dd17; 0xf70e5939; 0xffc00b31; 0x68581511; 0x64f98fa7; 0xbefa4fa4] // second 32 bits of the fractional parts of the square roots of the 9th through 16th primes 23..53
-  | SHA256 -> [0x6a09e667; 0xbb67ae85; 0x3c6ef372; 0xa54ff53a; 0x510e527f; 0x9b05688c; 0x1f83d9ab; 0x5be0cd19] // first 32 bits of the fractional parts of the square roots of the first 8 primes 2..19
-  | SHA384 -> [0xcbbb9d5dc1059ed8; 0x629a292a367cd507; 0x9159015a3070dd17; 0x152fecd8f70e5939; 0x67332667ffc00b31; 0x8eb44a8768581511; 0xdb0c2e0d64f98fa7; 0x47b5481dbefa4fa4]
-  | SHA512 -> [0x6a09e667f3bcc908; 0xbb67ae8584caa73b; 0x3c6ef372fe94f82b; 0xa54ff53a5f1d36f1; 0x510e527fade682d1; 0x9b05688c2b3e6c1f; 0x1f83d9abfb41bd6b; 0x5be0cd19137e2179]
-*)
 
-// core algorithm, accumulating an extra block into the current state
-assume val compress: #a:alg -> acc a -> lbytes (blockLen a) -> Tot (acc a)
-
-val hash2: #a:alg -> acc a -> b:bytes { length b % blockLen a = 0 } -> Tot (acc a) (decreases (length b))
-let rec hash2 #a v b = 
-  if length b = 0 then v 
-  else 
-    let c,b = split b (blockLen a) in 
-    hash2 (compress v c) b 
-
-assume val truncate: #a:alg -> acc a -> Tot (lbytes (tagLen a))
-
-// for convenience, we treat inputs as sequences of bytes, not bits. 
-// but note what's encoded in the suffix is the length in bits. 
-
-let suffixLen (a:alg) (len:nat) : n:nat {(n + len) % blockLen a = 0} = 
-  let lenlen = match a with | SHA384 | SHA512 -> 8 | _ -> 4 in 
-  let required = len + 1 + lenlen in // minimal length after padding and encoding the length
-  let zeros = // minimal extra padding for block alignment
-    if required % blockLen a = 0 then 0 else blockLen a - (required % blockLen a) in
-    //was, harder to prove: required + blockLen a - ((required - 1) % blockLen a + 1) in 
-  1 + zeros + lenlen
-
-// injective encoding for variable-length inputs
-// we add either 8 or 16 bytes of length and 1+ bytes of padding
-assume val suffix: a:alg -> len:nat -> Tot (c:lbytes (suffixLen a len))
-
-// computed in one step (specification) 
-val hash: a:alg -> bytes -> Tot (lbytes (tagLen a))
-let hash a b = 
-  let padded = b @| suffix a (length b) in 
-  let v = hash2 (acc0 a) padded in 
-  truncate v
+(* another PURE, VERIFIED, INCREMENTAL IMPLEMENTATION 
+    not usable yet, as we don't have a full F* specification 
+    of the underlying core algorithms, or their OpenSSL code.
 
 // an "outer" state for specifying incremental evaluation 
 // (we may additionally record the input bytestring)
-noeq type accv (a:alg) = | Acc: len:nat -> v:acc a -> b:lbytes (len % blockLen a) -> accv a 
+noeq type accv (a:alg) = | Acc: 
+    len:nat -> // total input length so far
+    v:acc a -> // current internal state 
+    b:lbytes (len % blockLen a) -> // pending bytes to be hashed  
+    accv a 
+
+// the real state for our pure reference implementation
+// the ideal state may keep instead the whole input bytestring
+// or we could index this type with the whole input bytestring
 
 // incremental computation (specification) 
 val hashA: a:alg -> bytes -> Tot (accv a)
@@ -141,13 +102,13 @@ let extend #a content v b =
   assert(hash2 v.v hashed == hash2 (acc0 a) (b0 @| hashed));
   Acc (v.len + length b) (hash2 v.v hashed) rest
 
-val finalize: 
+val final: 
   #a:alg -> 
   content:bytes (* TODO: ghost in real mode *) ->
   v:accv a { v == hashA a content } -> 
   Tot (t:lbytes (tagLen a) {t = hash a content})
   
-let finalize #a content v = 
+let final #a content v = 
   let b0, rest = split content (length content - length content % blockLen a) in 
   assert(Seq.equal content (b0 @| rest));
   let b1 = v.b @| suffix a v.len in 
@@ -156,114 +117,5 @@ let finalize #a content v =
   hash2_append (acc0 a) b0 b1; 
   truncate (hash2 v.v b1)
 
-
-
-
-(*
-//________________ Hash.OpenSSL.fsti (lax-coded in ML and C) __________________
-// towards a shared API for hashes; the code above provides a reference implenentation.
-
-assume type hash_ctx (a:alg) (r:rgn): Type0 
-assume val accT: #a:alg -> #r:rgn -> hash_ctx a r -> mem -> GTot (accv a)  // getting the spec out
-assume val accInv: #a:alg -> #r:region -> v:hash_ctx a r -> h0:mem -> h1:mem ->
-  Lemma(h0 `on` r == h1 `on` r  ==> accT v h0 == accvT v h1)
-
-assume val digest_create: a:alg -> parent:rgn -> ST (r:rgn & hash_ctx a r)
-  (requires (fun h -> True))
-  (ensures (fun h0 (r,v) h1 -> 
-    modifies Set.empty h0 h1 /\
-    extends r parent /\
-    stronger_fresh_region r h0 h1 /\
-    accT v h1 == start a ))
-    
-assume val digest_update: #a:alg -> #r:rgn -> v:hash_ctx a r -> b:bytes -> ST unit 
-  (requires (fun h -> True))
-  (ensures (fun h0 () h1 ->
-    modifies_one r h0 h1 /\
-    accT v h1 == extend (accT v h0) b))
-
-assume val digest_final: #a:alg -> #r:rgn -> v:hash_ctx a r -> b:bytes -> ST (lbytes (tagLen a)) 
-  (requires (fun h -> True))
-  (ensures (fun h0 t h1 -> 
-    modifies_one r h0 h1 /\
-    t = finalize (accT v h0))) // not specifying the post accT makes v non-reusable
 *)
 
-
-(* TBC 
-//________________ Hash.Spec.CRF __________________
-
-// witnessing that we hashed this particular content (for collision detection)
-// to be replaced by a witness of inclusion in a global table of all hash computations.
-// (not sure how to manage that table)
-assume val hashed: bytes -> Type 
-
-// Hash.table: strong invariants: hash is injective on its contents.
-// witnessed(fun h -> sel h Hash.table `contains` b)
-
-// We keep a copy of the whole input bytestring to be recorded at the end of the hash.
-// This is a first "instrumentation" step in the crypto proof.
-
-val finalizeCR: 
-  #a:alg -> 
-  content:bytes (* TODO: ghost in real mode *) ->
-  v:accv { v == hashA a content } -> 
-  ST (lbytes (tagLen a))
-  (requires (fun h0 -> True))
-  (ensures (fun h0 t h1 -> 
-    t = hash content /\ 
-    hashed content /\
-    h0 == h1 
-    // TBC, e.g. 
-    // modifies_one h0 h1 hashTable /\ sel h1 hashTable == snoc (sel h0 hashTable) (content, t)
-  ))
-
-val stop: s:string -> ST 'a 
-  (requires (fun h -> True))
-  (ensures (fun h0 r h1 -> False))
-let rec stop (s:string) = stop s 
-
-let finalizeCR #a content v = 
-  let h = finalize content v in 
-  // do we have a collision?
-  let log = !hashTable in 
-  if Seq.forall (fun c -> h = hash a c => c = content)  log
-  then (hashTable := Seq.snoc log content; h) 
-  else stop "hash collision detected" 
-
-
-(*
-val collision_resistant: c0: bytes -> c1: bytes { hashed c0 /\ hashed c1 } -> ST unit 
-  (requires (fun h0 -> True))
-  (ensures (hash c0 = hash c1 ==> c0 = c1))
-let collision_resistant c0 c1 =
-  testify(hashed c0);
-  testify(hashed c1);
-  let current = !Hash.table in 
-  ()
-*)
-
-*)
-
-
-
-(*
-(* Parametric hash algorithm (implements interface) *)
-val hash': hashAlg -> bytes -> Tot bytes
-let hash' alg data: bytes =
-    match alg with
-    | NULL    -> data
-    | MD5SHA1 -> (CoreCrypto.hash MD5 data) @| (CoreCrypto.hash SHA1 data)
-    | Hash h  -> (CoreCrypto.hash h  data)
-
-val hash: hashAlg -> bytes -> Tot bytes
-let hash alg data: bytes =
-  let h = hash' alg data in
-  let l = length h in
-    h
-(*
-  let exp = hashSize alg in
-  if l = exp then h
-  else Platform.Error.unexpected "CoreCrypto.Hash returned a hash of an unexpected size"
-*)
-*)
