src/tls/Hashing.CRF.fst
@@ -1,0 +1,92 @@
+﻿(** computational assumption: collision resistance *)
+module Hashing.CRF
+
+open FStar.Heap
+open FStar.HyperHeap
+open FStar.HyperStack
+
+open Platform.Bytes
+open Hashing.Spec
+
+assume val crf: alg -> Tot bool  // to be moved elsewhere, set to false for real extraction
+
+(* Depending on a single, global idealization function, we keep a global
+    table of all (finalized) hash computations, and we use it to
+    detect concrete collisions. Technically, this is modelled as
+    non-termination of a stateful, partially-correct finalize filter.
+    This may depend on some prior flag to keep the hashed input in the
+    incremental hash implementation. (This is always the case for now.)  *)
+
+module MR = FStar.Monotonic.RRef
+module MM = MonotoneMap
+
+// the precise types guarantee that the table stays empty when crf _ = false
+type range = | Computed: a: alg {crf a} -> tag a -> range
+type domain = fun (Computed a t) -> b:bytes { Seq.equal (hash a b) t }
+
+let inv (f:MM.map' range domain) = True 
+
+(* avoiding:
+  // when computed, f is injective on each collision-resistant algorithm
+  forall (a:alg{crf a}) (b0:bytes) (b1:bytes). 
+    ( match f (a,b0), f(a,b1) with 
+      | Some h0, Some h1 -> Seq.equal h0 h1 ==> Seq.equal b0 b1 
+      | _ -> True *)
+
+let table = MM.alloc #TLSConstants.tls_tables_region #range #domain #inv
+
+
+// witnessing that we hashed this particular content (for collision detection)
+// to be replaced by a witness of inclusion in a global table of all hash computations.
+// (not sure how to manage that table)
+
+//val hashed: a:alg -> b:bytes -> Type
+abstract type hashed a b = 
+  crf a ==> (
+    let h = hash a b in 
+    let b: domain (Computed a h) = b in 
+    MR.witnessed (MM.contains table (Computed a h) b))
+
+val crf_injective (a:alg) (b0:bytes) (b1:bytes): ST unit 
+  (requires (fun h0 -> hashed a b0 /\ hashed a b1 /\ Seq.equal (hash a b0) (hash a b1)))
+  (ensures (fun h0 _ h1 -> crf a ==> Seq.equal b0 b1))
+let crf_injective a b0 b1 =
+  if crf a then (
+    MR.m_recall table;
+    let f = MR.m_read table in
+    let h = hash a b0 in 
+    MR.testify(MM.contains table (Computed a h) b0);
+    MR.testify(MM.contains table (Computed a h) b1);
+  ())
+
+val stop: s:string -> ST 'a 
+  (requires (fun h -> True))
+  (ensures (fun h0 r h1 -> False))
+let rec stop (s:string) = stop s 
+
+open Hashing
+val finalize: 
+  #a:alg -> 
+  v:accv a -> 
+  ST (lbytes (tagLen a))
+  (requires (fun h0 -> True))
+  (ensures (fun h0 t h1 -> 
+    //TODO modifies table /\
+    let b = content v in 
+    t = hash a b /\ hashed a b 
+  ))
+
+let finalize #a v = 
+  let b = Hashing.content v in 
+  let h = Hashing.finalize v in 
+  if crf a then 
+    let x = Computed a h in 
+    ( match MM.lookup table x with 
+      | None -> MM.extend table x b; h
+      | Some b' -> 
+          if b = b' then h 
+          else stop "hash collision detected" )
+  else h
+
+
+
